vale/code/arch/x64/Vale.X64.Decls.fst
@@ -59,6 +59,14 @@ let va_opr_lemma_Mem128 s base offset t b index =
   assert (valid_buf_maddr128 (eval_maddr m s) h s.vs_memTaint b index t 0); // TODO HEAPLET
   M.lemma_load_mem128 b index h
 
+let va_opr_lemma_Mem128h s hi base offset t b index =
+  let h = M.get_vale_heap s.vs_heap in
+  let t = va_opr_code_Mem128h hi base offset t in
+  M.lemma_valid_mem128 b index h;
+  let OMem (m, t, _) = t in
+  assert (valid_buf_maddr128 (eval_maddr m s) h s.vs_memTaint b index t hi);
+  M.lemma_load_mem128 b index h
+
 let taint_at memTaint addr = Map.sel memTaint addr
 
 let va_cmp_eq o1 o2 = BC.OEq o1 o2
