vale/code/arch/x64/interop/Vale.Wrapper.X64.GCMencryptOpt.fst
@@ -1,5 +1,5 @@
 module Vale.Wrapper.X64.GCMencryptOpt
-
+(*
 open FStar.Mul
 open Vale.Stdcalls.X64.GCMencryptOpt
 open Vale.AsLowStar.MemoryHelpers
@@ -204,7 +204,6 @@ inline_for_extraction
 let gcm128_encrypt_opt' key iv auth_b auth_bytes auth_num keys_b iv_b hkeys_b abytes_b
   in128x6_b out128x6_b len128x6 in128_b out128_b len128_num inout_b plain_num scratch_b tag_b =
 
-assume False;
   let h0 = get() in
 
   B.disjoint_neq iv_b auth_b;
@@ -998,3 +997,4 @@ let gcm128_encrypt_opt_stdcall key iv plain_b plain_len auth_b auth_len iv_b out
     Seq.equal (seq_uint8_to_seq_nat8 (B.as_seq h2 tag_b)) tag);
 
   pop_frame()
+*)
