vale/specs/hardware/Vale.X64.Print_s.fst
@@ -232,6 +232,7 @@ let print_ins (ins:ins) (p:printer) : string =
   | Pop dst _      -> p.ins_name "  pop"  [dst] ^ print_operand dst p
   | Alloc n       -> p.ins_name "  sub" [OReg rRsp; OConst n] ^ print_ops (OReg rRsp) (OConst n)
   | Dealloc n       -> p.ins_name "  add" [OReg rRsp; OConst n] ^ print_ops (OReg rRsp) (OConst n)
+  | SetHeapletMap _ _ _ -> ""
 
 let print_cmp (c:ocmp) (counter:int) (p:printer) : string =
   let print_ops (o1:operand64) (o2:operand64) : string =
